lean_impl/AptpCheck.lean
@@ -16,6 +16,7 @@ import AptpCheck.Model.EncodingSound
 import AptpCheck.Model.NetworkMLP
 import AptpCheck.Cert.Vipr
 import AptpCheck.Cert.ViprFlat
+import AptpCheck.Cert.ViprSem
 import AptpCheck.Ast.Vipr
 import AptpCheck.Ast.NetRoundtrip
 import AptpCheck.Ast.AptpRoundtrip
